Start fixing globals and package initialization to work better with
multiple packages.

new/golang/defn/globals.v
@@ -1,7 +1,7 @@
 From New.golang.defn Require Import mem typing list pkg.
 From Perennial Require Import base.
 
-Module globals.
+Module option.
 Section defns.
 Context `{ffi_syntax}.
 
@@ -13,23 +13,32 @@ Definition unwrap_def : val :=
 Program Definition unwrap := sealed @unwrap_def.
 Definition unwrap_unseal : unwrap = _ := seal_eq _.
 
+End defns.
+End option.
+
+Module globals.
+Section defns.
+Context `{ffi_syntax}.
+
 Definition get_def : val :=
-  λ: "pkg_name" "var_name",
-    let: (("varAddrs", "functions"), "typeToMethodSets") := unwrap $ GlobalGet "pkg_name" in
-    unwrap $ alist_lookup "var_name" "varAddrs".
+  λ: "var_name", match: alist_lookup "var_name" (option.unwrap $ GlobalGet "__global_vars") with
+                   NONE => #null
+                 | SOME "v" => "v"
+                 end .
 Program Definition get := sealed @get_def.
 Definition get_unseal : get = _ := seal_eq _.
 
-(* XXX: unsealed because user has to prove WPs for this by unfolding. *)
+(* Allocates variables *just* for a single package. Unsealed because user proves
+   WPs for this by unfolding. *)
 Definition alloc (vars : list (go_string * go_type)) : val :=
   λ: <>, (fix alloc (vars : list (go_string * go_type)) : expr :=
            (match vars with
             | Datatypes.nil => alist_val []
             | (pair name t) :: vars =>
                 list.Cons (#name, mem.alloc (zero_val t)) (alloc vars)
-            end)%E) vars
-.
+            end)%E) vars.
 
+(* FIXME: *)
 Definition package_init_def (pkg_name : go_string) `{!PkgInfo pkg_name} : val :=
   let functions_val := alist_val (pkg_functions pkg_name) in
   let msets_val := alist_val ((λ '(name, mset), (name, alist_val mset)) <$> (pkg_msets pkg_name)) in
@@ -55,17 +64,17 @@ Context `{ffi_syntax}.
 Definition func_call_def : val :=
   λ: "pkg_name" "func_name",
     (λ: "firstArg",
-    let: (("varAddrs", "functions"), "typeToMethodSets") := globals.unwrap $ GlobalGet "pkg_name" in
-    (globals.unwrap $ alist_lookup "func_name" "functions") "firstArg").
+    let: (("varAddrs", "functions"), "typeToMethodSets") := option.unwrap $ GlobalGet "pkg_name" in
+    (option.unwrap $ alist_lookup "func_name" "functions") "firstArg").
 Program Definition func_call := sealed @func_call_def.
 Definition func_call_unseal : func_call = _ := seal_eq _.
 
 Definition method_call_def : val :=
   λ: "pkg_name" "type_name" "method_name" "receiver",
     (λ: "firstArg",
-       let: (("varAddrs", "functions"), "typeToMethodSets") := globals.unwrap $ GlobalGet "pkg_name" in
-       let: "methodSet" := globals.unwrap $ alist_lookup "type_name" "typeToMethodSets" in
-       (globals.unwrap $ alist_lookup "method_name" "methodSet") "receiver" "firstArg"
+       let: (("varAddrs", "functions"), "typeToMethodSets") := option.unwrap $ GlobalGet "pkg_name" in
+       let: "methodSet" := option.unwrap $ alist_lookup "type_name" "typeToMethodSets" in
+       (option.unwrap $ alist_lookup "method_name" "methodSet") "receiver" "firstArg"
     ).
 Program Definition method_call := sealed @method_call_def.
 Definition method_call_unseal : method_call = _ := seal_eq _.
